change DConcat to allow any permutation of the contents
previously was forcing the bits satisfying the first assertion to come
before the bits satisfying the second.

this allows me to prove the sanity tests t12 and t13.

sslScript.sml
@@ -1,4 +1,4 @@
-open HolKernel bossLib boolLib boolSimps Parse lcsymtacs stringTheory intLib finite_mapTheory ParseExtras
+open HolKernel bossLib boolLib boolSimps Parse lcsymtacs stringTheory intLib finite_mapTheory sortingTheory listTheory ParseExtras
 
 val _ = new_theory"ssl"
 
@@ -244,7 +244,7 @@ val DExp_def = Define`
 
 val DConcat_def = Define`
   DConcat (da1:dir_assertion) (da2:dir_assertion) =
-    { l1++l2 | l1 ∈ da1 ∧ l2 ∈ da2 }`
+    { ds | ∃l1 l2. l1 ∈ da1 ∧ l2 ∈ da2 ∧ PERM (l1++l2) ds }`
 val _ = overload_on("+",``DConcat``)
 
 val DContextApplication_def = Define`
@@ -843,14 +843,29 @@ val t12 = prove(
     simp[Once eval_prog_exp_cases] ) >>
   srw_tac[DNF_ss][] >>
   simp[Once eval_exp_cases] >>
-  simp[Once eval_prog_exp_cases] )
+  simp[Once eval_prog_exp_cases] >>
+  qho_match_abbrev_tac`∃l2 ds. PERM (D ds::l2) (CONS (D []) Y)` >>
+  `D [] :: Y = [] ++ (D [] :: Y)` by simp[] >>
+  pop_assum SUBST1_TAC >>
+  qexists_tac`Y` >> qexists_tac`[]` >>
+  match_mp_tac CONS_PERM >>
+  simp[])
 
 (* + is commutative *)
-(* Ramana: this is false too! *)
 val t13 = prove(
-  ``^dir ∈ (DDir (Name "a") (DDir (Name "c") T) + T)``,
-  rw[DDirectory_def,DConcat_def] >>
-  srw_tac[DNF_ss][])
+  ``^dir ∈ (DDir (Name "a") ((DDir (Name "c") T) + T))``,
+  rw[DDirectory_def,DConcat_def] >- (
+    simp[Once eval_exp_cases] >>
+    simp[Once eval_prog_exp_cases] ) >>
+  srw_tac[DNF_ss][] >>
+  simp[Once eval_exp_cases] >>
+  simp[Once eval_prog_exp_cases] >>
+  qho_match_abbrev_tac`∃l2 ds. PERM (D ds::l2) (CONS E (CONS (D X) Y))` >>
+  qexists_tac`E::Y` >> qexists_tac`X` >>
+  `E::D X::Y = [E] ++ D X :: Y` by simp[] >>
+  pop_assum SUBST1_TAC >>
+  match_mp_tac CONS_PERM >>
+  simp[])
 
 (*
 val subst_forest_MAP = store_thm("subst_forest_MAP",
